added annotations in term and subst;

subst.fst
@@ -4,11 +4,21 @@ open Term
 
 type subst = list (variable * term)
 
+(** Checks whether the substitution is cyclic or not   **)
 val isnt_cyclic : subst -> Tot bool
+
+(** Returns the list of the terms in the substitution the variables are mapped to**)
 val get_Images : subst -> Tot (list term)
+
+(** Returns the Domain of the substitution**)
 val get_Domain : subst -> Tot (list variable)
+
+(**Checks whether any variable in the first argument is present in
+    any of the terms in the second argument or not.
+    Returns true if no variable is present in any of the terms**)
 val check_presence_vars_in_terms : list variable -> list term -> Tot bool
 
+(**Checks whether the element is present in the list or not**)
 val mem: #a:eqtype -> a -> list a -> Tot bool
 let rec mem #a x xs = match xs with
   | [] -> false
@@ -26,6 +36,7 @@ let rec check_presence_vars_in_terms lv lt = match lv with
   | [] -> true
   | hd::tl -> not(is_var_present_list hd lt) && (check_presence_vars_in_terms tl lt)
 
+(**States that if the variables arent present in a list, they are not going to be present in a smaller list**)
 val aux_lemma1 : lv:list variable -> hd:term -> tl:list term -> Lemma
   (requires true)
   (ensures (check_presence_vars_in_terms lv (hd::tl)) ==> (check_presence_vars_in_terms lv tl) )
@@ -38,15 +49,19 @@ let isnt_cyclic st =
   let lt = get_Images st in
   check_presence_vars_in_terms lv lt
 
+(**States that if a substitution isnt cyclic then a sub-list substitution isnt cyclic too**)
 val aux_lemma2 : hd:(variable*term) -> tl:subst -> Lemma
   (requires true)
   (ensures isnt_cyclic (hd::tl) ==> isnt_cyclic tl )
 
 let aux_lemma2 hd tl = aux_lemma1 (get_Domain tl) (snd hd) (get_Images tl)
 
+(** The function that applies the substitution to a term.
+    apply_list is the companion function for doing the same to lists**)
 val apply : subst -> term ->Tot term
 val apply_list : subst -> l1:list term ->Tot (l2:list term{FStar.List.Tot.length l1 = FStar.List.Tot.length l2})
 
+(**Returns the term that the input variable corresponds to in the substitution**)
 val get_Term : v:variable -> s:subst{ mem v (get_Domain s) } -> Tot term
 
 let rec get_Term v st= match st with
@@ -60,12 +75,15 @@ let rec apply st t = match t with
   | [] -> []
   | hd::tl -> (apply st hd)::(apply_list st tl)
 
+(**Checks whether the input lists have a common element or not.
+   Returns true if there is no common element**)
 val distinct_lists : #a:eqtype -> list a -> list a -> Tot bool
 
 let rec distinct_lists #a l1 l2 = match l1 with
   | [] -> true
   | hd::tl -> not(mem hd l2) && (distinct_lists tl l2)
 
+(**Checks whether the input substitutions have non-overlapping domains or not**)
 val distinct_domain: subst -> subst -> Tot bool
 
 let distinct_domain st1 st2 =
@@ -73,24 +91,29 @@ let distinct_domain st1 st2 =
   let dom2 = get_Domain st2 in
   distinct_lists dom1 dom2
 
+(**Checks whether the 2 input substitutions are composable or not.**)
 val is_composable : subst -> subst -> Tot bool
 
 let is_composable st1 st2 = (distinct_domain st1 st2)
                             && isnt_cyclic st1 && isnt_cyclic st2
                             && check_presence_vars_in_terms (get_Domain st1) (get_Images st2)
 
+(**States that if hd::tl and st2 are composable then tl and st2 are composable too**)
 val aux_lemma3 : hd:(variable*term) -> tl:subst -> st:subst -> Lemma
   (requires is_composable (hd::tl) st)
   (ensures is_composable tl st)
 
 let rec aux_lemma3 hd tl st = aux_lemma2 hd tl
 
+(**Returns the composition of two substitutions**)
 val compose : st1:subst -> st2:subst -> Tot subst
 
 let rec compose st1 st2 = match st1 with
   | [] -> st2
   | hd::tl -> (fst hd,apply st2 (snd hd))::(compose tl st2)
 
+(**Returns whether the 2 substitutions are equivalent under application or not.
+  Is different from equality as order here is unimportant.**)
 val is_equal : #a:eqtype -> list a -> list a -> Tot bool
 
 let is_equal #a l1 l2 = (FStar.List.Tot.subset l1 l2) && (FStar.List.Tot.subset l2 l1)
@@ -101,7 +124,7 @@ val is_unify : term -> term -> bool
 
 val mgs : t1:term -> t2:term{ is_unify t1 t2 } -> subst*)
 
-
+(**States that the application of a substitutions on a ground term returns the same term **)
 val ground_term_lemma : st:subst -> t:term -> Lemma (requires (is_ground t)) (ensures (apply st t)=t)
 val ground_list_term_lemma : st:subst -> lt:list term -> Lemma
   (requires (is_ground_list lt))
@@ -114,6 +137,9 @@ let rec ground_term_lemma st t = match t with
   | [] -> ()
   | hd::tl -> (ground_term_lemma st hd) ; (ground_list_term_lemma st tl)
 
+(**Auxiliary lemma for compose_lemma.
+  States that the domain of composition of 2 composable substitutions is the
+  union of the domains of the substitutions. **)
 val compose_aux_lemma1 : st1:subst -> st2:subst -> Lemma
   (requires (is_composable st1 st2))
   (ensures forall (x:variable).
@@ -126,6 +152,10 @@ let rec compose_aux_lemma1 st1 st2 = match st1 with
   | [] -> ()
   | hd::tl -> aux_lemma3 hd tl st2 ; compose_aux_lemma1 tl st2
 
+(**Auxiliary lemma for compose_lemma.
+  States that the term corresponding to a variable v in composition of st1 and st2 is
+  either the application of st2 to a term in st1 to which v corresponds to
+  or the term in st2 itself which v corresponds to.  **)
 val compose_aux_lemma2 : st1:subst -> st2:subst -> x:variable -> Lemma
  (requires (is_composable st1 st2))
  (ensures ( (mem x (get_Domain st1) ==> mem x (get_Domain (compose st1 st2)) /\ (get_Term x (compose st1 st2) = apply st2 (get_Term x st1))) /\
@@ -136,6 +166,10 @@ let rec compose_aux_lemma2 st1 st2 x = match st1 with
   | hd::tl -> if x=fst hd then () else
     (aux_lemma3 hd tl st2 ; compose_aux_lemma1 st1 st2; compose_aux_lemma2 tl st2 x)
 
+(**composition lemma.
+  States that the application of composition of two substitutions is equal to
+  the substitutions applied in succession.
+  compose_list_lemma is the corresponding lemma for lists**)
 val compose_lemma : st1:subst -> st2:subst -> t:term -> Lemma
   (requires is_composable st1 st2)
   (ensures apply (compose st1 st2) t= apply st2 (apply st1 t))
@@ -158,13 +192,19 @@ let rec subset_lemma #a e l = match l with
   | [] -> ()
   | hd::tl -> subset_lemma hd tl ; subset_lemma e (hd::tl)*)
 
-val commutation_aux_lemma2 : st1:subst -> st2:subst -> Lemma
-  (requires isnt_cyclic (FStar.List.tot.append st1 st2))
-  (ensures ( (compose st1 st2) = (FStar.List.tot.append st1 st2) ) )
+val commutation_aux_lemma2 : hd:(variable*term) -> tl:subst -> Lemma
+  (requires isnt_cyclic (hd::tl))
+  (ensures (apply tl (snd hd) = (snd hd)) )
 
-let rec commutation_aux_lemma2 st1 st2 = match st1 with
+let commutation_aux_lemma2 hd tl = ()
+
+(*val commutation_aux_lemma3 : st1:subst -> st2:subst -> Lemma
+  (requires isnt_cyclic (FStar.List.Tot.append st1 st2))
+  (ensures ( (compose st1 st2) = (FStar.List.Tot.append st1 st2) ) )
+
+let rec commutation_aux_lemma3 st1 st2 = match st1 with
   | [] -> ()
-  | hd::tl -> commutation_aux_lemma2 tl st2
+  | hd::tl -> aux_lemma2 hd (FStar.List.Tot.append tl st2); commutation_aux_lemma3 tl st2*)
 
 (*val commutation_aux_lemma1 : #a:eqtype -> e1:a -> e2:a -> l:list a-> Lemma
   (requires true)
